

Para la coadición

$$f_3(q)^2 + f(x_0) + (x - x_0) \cdot f[x_1, x_0] + (x - x_0)(x - x_1) \cdot f[x_2, x_1, x_0]$$

$$+ (x - x_0)(x - x_1)(x - x_2) \cdot f[x_3, x_2, x_1, x_0]$$

$$+ [x_3, x_2, x_1, x_0] = \frac{f[x_3, x_2, x_1, x_0] - f[x_3, x_2, x_0]}{x_3 - x_0}$$

$$= \frac{f(x_3, x_1) - f(x_2, x_1)}{x_3 - x_1} - \frac{f(x_3, x_0) - f(x_2, x_0)}{x_3 - x_0}$$

$$= \frac{\frac{f(x_3) - f(x_1)}{x_3 - x_1} - \frac{f(x_2) - f(x_1)}{x_2 - x_1}}{x_3 - x_1} - \frac{\frac{f(x_3) - f(x_0)}{x_3 - x_1} - \frac{f(x_2) - f(x_0)}{x_2 - x_0}}{x_3 - x_0}$$

$$\Rightarrow \underline{f[x_1, x_0]} = \frac{f(x_1) - f(x_0)}{x_1 - x_0} = \frac{1,386294 - 0}{4 - 1} = \underline{0,462098}$$

$$\Rightarrow \underline{f[x_2, x_1, x_0]} = \frac{\frac{f(x_2) - f(x_1)}{x_2 - x_1} - \frac{f(x_1) - f(x_0)}{x_1 - x_0}}{x_2 - x_0} = \underline{-0,0597385}$$

$$\Rightarrow \underline{f[x_3, x_2, x_1, x_0]} = \frac{\frac{0,182314 - 0,223144}{6 - 4} - \frac{0,223144 - 0,407381}{6 - 1}}{6 - 1} = \underline{0,023594}$$

$$\underline{f[x_2, x_1, x_0]} = \frac{0,023594}{6 - 1} = \underline{0,0047188}$$

$$\Rightarrow \underline{f(2)} = \underline{0,609888/}$$

$$\underline{f[x_3, x_2, x_1, x_0]} = \frac{-0,020415 - (-0,044009)}{6 - 1} =$$